move encrypt, decrypt specs to interface

src/tls/Crypto.AEAD.fst
@@ -74,33 +74,7 @@ let footprint (#a: SC.supported_alg) (#phi: plain_pred) (h: HS.mem) (s: state a 
     EC.footprint h (state_ec s)
 
 let encrypt
-  (#a: SC.supported_alg)
-  (#phi: plain_pred)
-  (s: state a phi) // key
-  (plain: EC.plain_p a)
-  (plain_len: U32.t {U32.v plain_len == B.length plain})
-  (cipher: EC.cipher_p a) // cipher == iv ++ cipher ++ tag (see EverCrypt.AEAD.encrypt_st)
-: HST.Stack EE.error_code
-  (requires (fun h ->
-    invariant h s /\
-    B.live h plain /\
-    B.live h cipher /\
-    phi (B.as_seq h plain) /\
-    B.loc_disjoint (footprint h s) (B.loc_buffer plain) /\
-    B.loc_disjoint (footprint h s) (B.loc_buffer cipher) /\
-    B.disjoint plain cipher /\
-    B.length cipher == B.length plain + 12 + SC.tag_length a
-  ))
-  (ensures (fun h res h' -> 
-    match res with
-    | EE.InvalidKey ->
-      B.modifies B.loc_none h h'
-    | EE.Success ->
-      footprint h' s == footprint h s /\
-      B.modifies (B.loc_union (footprint h s) (B.loc_buffer cipher)) h h' /\
-      invariant h' s
-    | _ -> False
-  ))
+  #a #phi s plain plain_len cipher
 = let iv_len = 12ul in
   let iv = B.sub cipher 0ul iv_len in
   // E.random_sample iv_len iv;
@@ -126,33 +100,7 @@ let encrypt
   res
 
 let decrypt
-  (#a: SC.supported_alg)
-  (#phi: plain_pred)
-  (#s: state a phi) // key
-  (cipher: EC.cipher_p a) // cipher == iv ++ cipher ++ tag (see EverCrypt.AEAD.encrypt_st)
-  (cipher_len: U32.t { U32.v cipher_len == B.length cipher })
-  (plain: EC.plain_p a)
-: HST.Stack EE.error_code
-  (requires (fun h ->
-    invariant h s /\
-    B.live h plain /\
-    B.live h cipher /\
-    B.length cipher == B.length plain + 12 + SC.tag_length a /\
-    B.loc_disjoint (footprint h s) (B.loc_buffer plain) /\
-    B.loc_disjoint (footprint h s) (B.loc_buffer cipher) /\
-    B.disjoint plain cipher
-  ))
-  (ensures (fun h res h' ->
-    match res with
-    | EE.InvalidKey ->
-      B.modifies B.loc_none h h'
-    | EE.Success
-    | EE.AuthenticationFailure ->
-      B.modifies (B.loc_union (footprint h s) (B.loc_buffer plain)) h h' /\
-      footprint h' s == footprint h s /\
-      invariant h' s
-    | _ -> False
-  ))
+  #a #phi s cipher cipher_len plain
 = let iv_len = 12ul in
   let iv = B.sub cipher 0ul iv_len in
   let ad = B.sub iv 0ul 0ul in
