src/tls/Crypto.AEAD.fsti
@@ -19,6 +19,11 @@ type plain_pred = (plain: Seq.seq SC.uint8) -> Tot Type0
 inline_for_extraction
 val state (a: SC.supported_alg) (phi: plain_pred) : Tot Type0
 
+val state_kv
+  (#a: SC.supported_alg) (#phi: plain_pred)
+  (s: state a phi)
+: GTot (SC.kv a)
+
 val invariant (#a: SC.supported_alg) (#phi: plain_pred) (h: HS.mem) (s: state a phi) : GTot Type0
 
 val footprint (#a: SC.supported_alg) (#phi: plain_pred) (h: HS.mem) (s: state a phi) : GTot B.loc
@@ -35,3 +40,61 @@ let tag_len : (x: SC.alg) -> Tot (y: U32.t { U32.v y == SC.tag_length x }) =
   | CHACHA20_POLY1305 -> 16ul
   | AES128_CCM        -> 16ul
   | AES256_CCM        -> 16ul
+
+val encrypt
+  (#a: SC.supported_alg)
+  (#phi: plain_pred)
+  (s: state a phi) // key
+  (plain: EC.plain_p a)
+  (plain_len: U32.t {U32.v plain_len == B.length plain})
+  (cipher: EC.cipher_p a) // cipher == iv ++ cipher ++ tag (see EverCrypt.AEAD.encrypt_st)
+: HST.Stack EE.error_code
+  (requires (fun h ->
+    invariant h s /\
+    B.live h plain /\
+    B.live h cipher /\
+    phi (B.as_seq h plain) /\
+    B.loc_disjoint (footprint h s) (B.loc_buffer plain) /\
+    B.loc_disjoint (footprint h s) (B.loc_buffer cipher) /\
+    B.disjoint plain cipher /\
+    B.length cipher == B.length plain + 12 + SC.tag_length a
+  ))
+  (ensures (fun h res h' -> 
+    match res with
+    | EE.InvalidKey ->
+      B.modifies B.loc_none h h'
+    | EE.Success ->
+      footprint h' s == footprint h s /\
+      B.modifies (B.loc_union (footprint h s) (B.loc_buffer cipher)) h h' /\
+      invariant h' s
+    | _ -> False
+  ))
+
+val decrypt
+  (#a: SC.supported_alg)
+  (#phi: plain_pred)
+  (s: state a phi) // key
+  (cipher: EC.cipher_p a) // cipher == iv ++ cipher ++ tag (see EverCrypt.AEAD.encrypt_st)
+  (cipher_len: U32.t { U32.v cipher_len == B.length cipher })
+  (plain: EC.plain_p a)
+: HST.Stack EE.error_code
+  (requires (fun h ->
+    invariant h s /\
+    B.live h plain /\
+    B.live h cipher /\
+    B.length cipher == B.length plain + 12 + SC.tag_length a /\
+    B.loc_disjoint (footprint h s) (B.loc_buffer plain) /\
+    B.loc_disjoint (footprint h s) (B.loc_buffer cipher) /\
+    B.disjoint plain cipher
+  ))
+  (ensures (fun h res h' ->
+    match res with
+    | EE.InvalidKey ->
+      B.modifies B.loc_none h h'
+    | EE.Success
+    | EE.AuthenticationFailure ->
+      B.modifies (B.loc_union (footprint h s) (B.loc_buffer plain)) h h' /\
+      footprint h' s == footprint h s /\
+      invariant h' s
+    | _ -> False
+  ))
